theories/L6_PCPS/hoisting.v
@@ -21,68 +21,68 @@ Close Scope Z_scope.
   * of function definitions. 
   *)
 Fixpoint erase_fundefs (e : exp) (defs : fundefs)
-         (f : exp * fundefs -> exp * fundefs) {struct e} : exp * fundefs :=
+         (f : exp * fundefs * nat -> exp * fundefs * nat) {struct e} : exp * fundefs * nat :=
   match e with
     | Econstr x  tag ys e' =>
-      erase_fundefs e' defs (fun p => let (e, defs) := p in
-                                      f (Econstr x tag ys e, defs))
+      erase_fundefs e' defs (fun p => let '(e, defs, n) := p in
+                                      f (Econstr x tag ys e, defs, n))
     | Ecase x tes =>
       fold_left
-        (fun (f : exp * fundefs -> exp * fundefs) (te : ctor_tag * exp) =>
+        (fun (f : exp * fundefs * nat -> exp * fundefs * nat) (te : ctor_tag * exp) =>
            fun p =>
              let (c, e) := te in
-             let (e1, defs1) := p in
+             let '(e1, defs1, n1) := p in
              erase_fundefs e defs1
                        (fun p2 =>
-                          let (e2, defs2) := p2 in
+                          let '(e2, defs2, n2) := p2 in
                           match e1 with
-                            | Ecase x' tes' =>
-                              f (Ecase x' ((c, e2) :: tes'), defs2)
-                            | _ => (* This should never match *)
-                              f (Ecase x [(c, e2)], defs2)
-                          end)) tes f (Ecase x [], defs)
+                          | Ecase x' tes' =>
+                            f (Ecase x' ((c, e2) :: tes'), defs2, max n1 n2)
+                          | _ => (* This should never match *)
+                            f (Ecase x [(c, e2)], defs2, max n1 n2)
+                          end)) tes f (Ecase x [], defs, 0)
     | Eproj x tag n y e' =>
       erase_fundefs e' defs (fun p =>
-                           let (e, defs) := p in
-                           f (Eproj x tag n y e, defs))
+                               let '(e, defs, m) := p in
+                               f (Eproj x tag n y e, defs, m))
     | Eletapp x g ft ys e' =>
       erase_fundefs e' defs (fun p =>
-                               let (e, defs) := p in
-                               f (Eletapp x g ft ys e, defs))
-
+                               let '(e, defs, n) := p in
+                               f (Eletapp x g ft ys e, defs, n))
+                    
     | Efun fdefs e' =>
       erase_fundefs e' defs (fun p =>
-                           let (e'', defs'') := p in
-                           erase_nested_fundefs fdefs e'' defs'' f)
+                               let '(e'', defs'', n) := p in
+                               erase_nested_fundefs fdefs e'' defs'' (fun p => let '(e, defs, m) := p in f (e, defs, 1 + max n m)))
     | Eapp g ft xs =>
-      f (Eapp g ft xs, defs)
+      f (Eapp g ft xs, defs, 0)
     | Eprim x prim ys e' =>
       erase_fundefs e' defs (fun p =>
-                           let (e', defs') := p in
-                           f (Eprim x prim ys e', defs'))
-    | Ehalt x => f (Ehalt x, defs) 
+                               let '(e', defs', n) := p in
+                               f (Eprim x prim ys e', defs', n))
+    | Ehalt x => f (Ehalt x, defs, 0) 
   end
 with erase_nested_fundefs (defs : fundefs) (e : exp) (hdefs : fundefs)
-                          (f : exp * fundefs -> exp * fundefs) {struct defs}
-     : exp * fundefs :=
+                          (f : exp * fundefs * nat -> exp * fundefs * nat) {struct defs}
+     : exp * fundefs * nat :=
        match defs with 
          | Fcons g t xs e' defs =>
            erase_nested_fundefs defs e hdefs
                                 (fun p1 =>
-                                   let (e1, defs1) := p1 in
+                                   let '(e1, defs1, n1) := p1 in
                                    erase_fundefs e' defs1
                                                  (fun p2 =>
-                                                    let (e2, defs2) := p2 in
-                                                    f (e1, Fcons g t xs e2 defs2)))
-         | Fnil => f (e, hdefs)
+                                                    let '(e2, defs2, n2) := p2 in
+                                                    f (e1, Fcons g t xs e2 defs2, max n1 n2)))
+         | Fnil => f (e, hdefs, 0)
   end.
 
 (** [exp_hoist e] moves all function definitions of [e] at the outermost level *)
 Definition exp_hoist (e : exp) :=
-  let (e, defs) := erase_fundefs e Fnil id in
+  let '(e, defs, n) := erase_fundefs e Fnil id in
   match defs with
-    | Fnil => e
-    | _ => Efun defs e
+  | Fnil => (e, n)
+    | _ => (Efun defs e, n)
   end.
 
 
@@ -92,7 +92,7 @@ Section CC.
   Definition closure_conversion_hoist (e : exp) (c: comp_data) : error exp * comp_data :=    
     let '(e'_err, c') := closure_conversion_top clo_tag e c in
     match e'_err with 
-    | Ret e' => (Ret (exp_hoist e'), c')
+    | Ret e' => (Ret (fst (exp_hoist e')), c')
     | Err str => (Err str, c')
     end.
 
@@ -101,90 +101,92 @@ End CC.
 (** [erase_fundefs e e' B] iff [e'] is [e] after erasing all the function 
   *  definition blocks and [B] is exactly the function definitions of [e] 
   *) 
-Inductive Erase_fundefs : exp -> exp -> fundefs -> Prop :=
+Inductive Erase_fundefs : exp -> exp -> fundefs -> nat (* number of hoisting steps *) -> Prop :=
 | Efun_erase :
-    forall e e' defs Be Bdefs Be_defs,
-      Erase_fundefs e e' Be ->
-      Erase_nested_fundefs defs Bdefs ->
+    forall e e' defs Be Bdefs Be_defs n m,
+      Erase_fundefs e e' Be n ->
+      Erase_nested_fundefs defs Bdefs m ->
       split_fds Be Bdefs Be_defs ->
-      Erase_fundefs (Efun defs e) e' Be_defs
+      Erase_fundefs (Efun defs e) e' Be_defs (1 + max n m)
 | Econstr_erase :
-    forall x t ys e e' B,
-      Erase_fundefs e e' B ->
+    forall x t ys e e' B n,
+      Erase_fundefs e e' B n ->
       Erase_fundefs (Econstr x t ys e)
-                  (Econstr x  t ys e') B
+                  (Econstr x  t ys e') B n
 | Ecase_nil_erase :
     forall x,
-      Erase_fundefs (Ecase x nil) (Ecase x nil) Fnil
+      Erase_fundefs (Ecase x nil) (Ecase x nil) Fnil 0
 | Ecase_cons_erase :
-    forall x c e e' tes tes' B B' B'',
-      Erase_fundefs (Ecase x tes) (Ecase x tes') B ->
-      Erase_fundefs e e' B' ->
+    forall x c e e' tes tes' B B' B'' n m,
+      Erase_fundefs (Ecase x tes) (Ecase x tes') B n ->
+      Erase_fundefs e e' B' m ->
       split_fds B B' B'' ->
-      Erase_fundefs (Ecase x ((c, e) :: tes)) (Ecase x ((c, e') :: tes')) B''
+      Erase_fundefs (Ecase x ((c, e) :: tes)) (Ecase x ((c, e') :: tes')) B'' (max n m)
 | Eproj_erase :
-    forall x tau N y e e' B,
-      Erase_fundefs e e' B ->
+    forall x tau N y e e' B n,
+      Erase_fundefs e e' B n ->
       Erase_fundefs (Eproj x tau N y e)
-                    (Eproj x tau N y e') B
+                    (Eproj x tau N y e') B n
 | Eletapp_erase :
-    forall x f tau ys e e' B,
-      Erase_fundefs e e' B ->
+    forall x f tau ys e e' B n,
+      Erase_fundefs e e' B n ->
       Erase_fundefs (Eletapp x f tau ys e)
-                    (Eletapp x f tau ys e') B
+                    (Eletapp x f tau ys e') B n
 | Eapp_erase :
     forall f ft xs,
-      Erase_fundefs (Eapp f ft xs) (Eapp f ft xs) Fnil
-| Eprim_erase :
+      Erase_fundefs (Eapp f ft xs) (Eapp f ft xs) Fnil 0
+| Eprim_erase n :
     forall x f ys e e' B,
-      Erase_fundefs e e' B ->
+      Erase_fundefs e e' B n ->
       Erase_fundefs (Eprim x f ys e)
-                    (Eprim x f ys e') B
+                    (Eprim x f ys e') B n
 | Ehalt_erase :
-    forall x, Erase_fundefs (Ehalt x) (Ehalt x) Fnil
-with Erase_nested_fundefs : fundefs -> fundefs -> Prop :=
+    forall x, Erase_fundefs (Ehalt x) (Ehalt x) Fnil 0
+with Erase_nested_fundefs : fundefs -> fundefs -> nat -> Prop :=
 | Fcons_erase :
-    forall f tau xs e e' defs B B' B'',
-      Erase_fundefs e e' B ->
-      Erase_nested_fundefs defs B' ->
+    forall f tau xs e e' defs B B' B'' n m,
+      Erase_fundefs e e' B n ->
+      Erase_nested_fundefs defs B' m ->
       split_fds B (Fcons f tau xs e' B') B'' ->
-      Erase_nested_fundefs (Fcons f tau xs e defs) B''
+      Erase_nested_fundefs (Fcons f tau xs e defs) B'' (max n m)
 | Fnil_erase :
-    Erase_nested_fundefs Fnil Fnil.
+    Erase_nested_fundefs Fnil Fnil 0.
 
 (** Correspondence between the inductive and the computational definitions of function definition erasure *)
 Lemma erase_fundefs_in_Erase_fundefs :
   (forall e B f,
-   exists e' B' B'',
-     erase_fundefs e B f = f (e', B') /\
+   exists e' B' B'' m,
+     erase_fundefs e B f = f (e', B', m) /\
      split_fds B B'' B' /\
-     Erase_fundefs e e' B'') /\
+     Erase_fundefs e e' B'' m) /\
   (forall defs e B f,
-    exists B' B'',
-      erase_nested_fundefs defs e B f = f (e, B') /\
+    exists B' B'' m,
+      erase_nested_fundefs defs e B f = f (e, B', m) /\
       split_fds B B'' B' /\
-      Erase_nested_fundefs defs B'').
-Proof.
+      Erase_nested_fundefs defs B'' m).
+Proof. 
   exp_defs_induction IHe IHl IHf; intros; simpl in *;
-  try (now edestruct IHe as [e' [B' [B'' [Heq [Hsplit Her]]]]];
-       repeat eexists; eauto; try rewrite Heq; try constructor; auto).
+  try (now edestruct IHe as [e' [B' [B'' [m [Heq [Hsplit Her]]]]]];
+       repeat eexists; eauto; try rewrite Heq; try constructor; eauto).
   - repeat eexists; eauto using split_fds_nil_l; repeat econstructor.
-  - edestruct IHl as [e1' [B1' [B1'' [Heq1 [Hspl1 Her1]]]]]. 
-    edestruct IHe as [e2' [B2' [B2'' [Heq2 [Hspl2 Her2]]]]].
+  - edestruct IHl as [e1' [B1' [B1'' [m [Heq1 [Hspl1 Her1]]]]]]. 
+    edestruct IHe as [e2' [B2' [B2'' [n [Heq2 [Hspl2 Her2]]]]]].
     rewrite Heq1, Heq2. clear Heq1 Heq2.
     edestruct split_fds_trans as [B3 [H1 H2]]; [apply Hspl1 | |]; eauto.
     inv Her1; repeat eexists; eauto; econstructor; eauto; econstructor; eauto.
-  - edestruct IHe as [e2 [B2 [B2' [Heq2 [Hspl2 Her2]]]]].
-    edestruct IHf as [B1 [B1' [Heq1 [Hspl1 Her1]]]]; subst.
+  - edestruct IHe as [e2 [B2 [B2' [m [Heq2 [Hspl2 Her2]]]]]].
+    edestruct IHf as [B1 [B1' [n [Heq1 [Hspl1 Her1]]]]]; subst.
     edestruct split_fds_trans as [B3 [H1 H2]] ; [ | apply Hspl1 |]; eauto.
-    repeat eexists. rewrite Heq2, Heq1; eauto. eauto. econstructor; eauto.
+    repeat eexists. rewrite Heq2, Heq1; eauto. eauto.    
+    econstructor; eauto.
   - repeat eexists; eauto using split_fds_nil_l; repeat econstructor.
   - repeat eexists; eauto using split_fds_nil_l; econstructor.
-  - edestruct IHf as [B1 [B1' [Heq1 [Hspl1 Her1]]]]; subst.
-    edestruct IHe as [e2 [B2 [B2' [Heq2 [Hspl2 Her2]]]]].
+  - edestruct IHf as [B1 [B1' [m [Heq1 [Hspl1 Her1]]]]]; subst.
+    edestruct IHe as [e2 [B2 [B2' [n [Heq2 [Hspl2 Her2]]]]]].
     edestruct split_fds_trans as [B3 [H1 H2]] ; [ apply Hspl1 | |]; eauto.
     repeat eexists. rewrite Heq1, Heq2; eauto.
-    constructor; eauto. econstructor; eauto. constructor; eauto.
+    constructor. eassumption. 
+    rewrite Max.max_comm. econstructor; eauto. econstructor; eauto.
     apply split_fds_sym; eauto.
   - repeat eexists; eauto using split_fds_nil_l; repeat econstructor.
 Qed.
@@ -246,11 +248,11 @@ Qed.
 (** If [Erase_fundefs e e' B] then there are no function definitions 
     in [e'] and [B] *)
 Lemma erase_fundefs_no_fun :
-  (forall e e' B,
-     Erase_fundefs e e' B ->
+  (forall e e' B m,
+     Erase_fundefs e e' B m ->
      no_fun e' /\ no_fun_defs B) /\
-  (forall B B',
-     Erase_nested_fundefs B B' ->
+  (forall B B' m,
+     Erase_nested_fundefs B B' m ->
      no_fun_defs B').
 Proof.
   exp_defs_induction IHe IHl IHf; intros; simpl;
@@ -285,13 +287,13 @@ Qed.
 
 
 Lemma Erase_fundefs_bound_var_mut :
-  (forall e e' B (Herase : Erase_fundefs e e' B),       
+  (forall e e' B m (Herase : Erase_fundefs e e' B m),
       bound_var e <--> bound_var e' :|: bound_var_fundefs B) /\
-  (forall B B' (Herase : Erase_nested_fundefs B B'),
+  (forall B B' m (Herase : Erase_nested_fundefs B B' m),
       bound_var_fundefs B <--> bound_var_fundefs B').
 Proof.
   exp_defs_induction IHe IHc IHB;
-    try (intros e' B Hr); try (intros B' Hr); inv Hr;
+    try (intros e' B m Hr); try (intros B' m Hr); inv Hr;
       try (now repeat normalize_bound_var; rewrite IHe; [| eassumption ];
            split; xsets).
   - repeat normalize_bound_var. sets.
@@ -316,14 +318,14 @@ Qed.
 
 
 Lemma Erase_fundefs_bound_var :
-  forall e e' B (Herase : Erase_fundefs e e' B),       
+  forall e e' B m (Herase : Erase_fundefs e e' B m),
     bound_var e <--> bound_var e' :|: bound_var_fundefs B.
 Proof.
   eapply Erase_fundefs_bound_var_mut.
 Qed.
 
 Lemma Erase_nested_fundefs_bound_var :
-  forall B B' (Herase : Erase_nested_fundefs B B'),
+  forall B B' m (Herase : Erase_nested_fundefs B B' m),
     bound_var_fundefs B <--> bound_var_fundefs B'.
 Proof.
   eapply Erase_fundefs_bound_var_mut.
@@ -331,32 +333,32 @@ Qed.
 
 Ltac bound_var_heq Hname :=
   match goal with
-  | [ H : Erase_fundefs _ _ _ |- _ ] =>
-    assert (Hname := Erase_fundefs_bound_var _ _ _ H)
+  | [ H : Erase_fundefs _ _ _ _ |- _ ] =>
+    assert (Hname := Erase_fundefs_bound_var _ _ _ _ H)
   end.
 
 Ltac bound_var_fundefs_heq Hname :=
   match goal with
-  | [ H : Erase_nested_fundefs _ _ |- _ ] =>
-    assert (Hname := Erase_nested_fundefs_bound_var _ _ H)
+  | [ H : Erase_nested_fundefs _ _ _ |- _ ] =>
+    assert (Hname := Erase_nested_fundefs_bound_var _ _ _ H)
   end.
 
 
 Lemma Erase_fundefs_unique_bindings_mut :
-  (forall e e' B (Herase : Erase_fundefs e e' B),
+  (forall e e' B m (Herase : Erase_fundefs e e' B m),
       unique_bindings e ->
       unique_bindings e' /\
       unique_bindings_fundefs B /\
       Disjoint _ (bound_var_fundefs B) (bound_var e')) /\
-  (forall B B' (Herase : Erase_nested_fundefs B B'),
+  (forall B B' m (Herase : Erase_nested_fundefs B B' m),
       unique_bindings_fundefs B ->
       unique_bindings_fundefs B').
 Proof.
   exp_defs_induction IHe IHc IHB;
-    try (intros e' B Hr Hun); try (intros B' Hr Hun); inv Hr;
+    try (intros e' B m Hr Hun); try (intros B' m Hr Hun); inv Hr;
       try (bound_var_heq Hbin); try (bound_var_fundefs_heq Hbin'). 
   - inv Hun. 
-    edestruct (IHe _ _ H5) as [Hun [Hunf Hdis]]; eauto. 
+    edestruct (IHe _ _ _ H6) as [Hun [Hunf Hdis]]; eauto. 
     split; [| split ].
     + constructor; eauto.
       intros Hc. eapply H1. eapply Erase_fundefs_bound_var_mut.
@@ -373,29 +375,29 @@ Proof.
     + sets.
   - normalize_bound_var.
     inv Hun.
-    edestruct (IHe _ _ H6) as [Hun' [Hunf' Hd']]; eauto. 
-    edestruct (IHc _ _ H5) as [Hun [Hunf Hd]]; eauto.
-    clear H6. bound_var_heq Hbin'.
+    edestruct (IHe _ _ _ H7) as [Hun' [Hunf' Hd']]; eauto. 
+    edestruct (IHc _ _ _ H6) as [Hun [Hunf Hd]]; eauto.
+    clear H7. bound_var_heq Hbin'.
     split; [| split ].
-    + constructor; eauto. 
-      eapply Disjoint_Included; [| | eapply H8 ].
+    + constructor; eauto.  
+      eapply Disjoint_Included; [| | eapply H5 ].
       rewrite Hbin'. sets.
       rewrite Hbin. sets.
     + rewrite Hbin', Hbin in *.  
       eapply split_fds_unique_bindings_fundefs_r;
         [| | | eassumption ]; eauto.
       eapply Disjoint_sym.
-      eapply Disjoint_Included; [| | eapply H8 ]; sets.
+      eapply Disjoint_Included; [| | eapply H5 ]; sets.
     + rewrite (split_fds_bound_vars B0 B' B); eauto.
       rewrite Hbin, Hbin' in *.
       eapply Union_Disjoint_l; eapply Union_Disjoint_r.
       * eapply Disjoint_sym.
-        eapply Disjoint_Included; [| | eapply H8 ]; sets.
+        eapply Disjoint_Included; [| | eapply H5 ]; sets.
       * eassumption.
       * eassumption.
-      * eapply Disjoint_Included; [| | eapply H8 ]; sets.
+      * eapply Disjoint_Included; [| | eapply H5 ]; sets.
   - inv Hun. 
-    edestruct (IHe _ _ H6) as [Hun [Hunf Hdis]]; eauto. 
+    edestruct (IHe _ _ _ H7) as [Hun [Hunf Hdis]]; eauto. 
     split; [| split ].
     + constructor; eauto.
       intros Hc. eapply H1. eapply Erase_fundefs_bound_var_mut.
@@ -406,7 +408,7 @@ Proof.
       eassumption. eapply Disjoint_Singleton_r.
       intros Hc. eapply H1. eapply Hbin. now right.
   - inv Hun.
-    edestruct (IHe _ _ H6) as [Hun [Hunf Hdis]]; eauto. 
+    edestruct (IHe _ _ _ H7) as [Hun [Hunf Hdis]]; eauto. 
     split; [| split ].
     + constructor; eauto.
       intros Hc. eapply H1. eapply Erase_fundefs_bound_var_mut.
@@ -417,12 +419,12 @@ Proof.
       eassumption. eapply Disjoint_Singleton_r.
       intros Hc. eapply H1. eapply Hbin. now right.
   - inv Hun.
-    edestruct (IHe _ _ H1) as [Hun [Hunf Hdis]]; eauto. 
-    assert (Hunf' := IHB _ H2 H4).
+    edestruct (IHe _ _ _ H1) as [Hun [Hunf Hdis]]; eauto. 
+    assert (Hunf' := IHB _ _ H2 H4).
     split; [| split ]; eauto.
     + eapply split_fds_unique_bindings_fundefs_r;
         [ | | | eassumption ]; eauto.
-      eapply Disjoint_Included; [| | eapply H6 ]; sets.
+      eapply Disjoint_Included; [| | eapply H5 ]; sets.
       rewrite Hbin'. sets.
       rewrite Hbin. sets.
     + erewrite (split_fds_bound_vars _ _ B); eauto.
@@ -430,7 +432,7 @@ Proof.
       * eassumption.
       * rewrite <- Hbin'.
         eapply Disjoint_sym.
-        eapply Disjoint_Included; [| | eapply H6 ]; sets.
+        eapply Disjoint_Included; [| | eapply H5 ]; sets.
         rewrite Hbin; sets.
   - inv Hun.
     split; [| split ]; eauto.
@@ -438,7 +440,7 @@ Proof.
     + constructor.
     + normalize_bound_var. sets.
   - inv Hun. 
-    edestruct (IHe _ _ H5) as [Hun [Hunf Hdis]]; eauto. 
+    edestruct (IHe _ _ _ H6) as [Hun [Hunf Hdis]]; eauto. 
     split; [| split ].
     + constructor; eauto.
       intros Hc. eapply H1. eapply Erase_fundefs_bound_var_mut.
@@ -460,7 +462,7 @@ Proof.
     * constructor; eauto.
       intros Hc; eapply H4. 
       eapply Hbin. now left.
-      intros Hc. eapply H8.
+      intros Hc. eapply H5.
       eapply Hbin'. eassumption.
       eapply Disjoint_Included_l; [| eapply H9 ]; sets.
       rewrite Hbin. sets.
@@ -485,30 +487,30 @@ Proof.
 Qed.
 
 Lemma Erase_nested_fundefs_name_in_fundefs :
-  (forall B B' (Herase : Erase_nested_fundefs B B'),
+  (forall B B' m (Herase : Erase_nested_fundefs B B' m),
       name_in_fundefs B \subset name_in_fundefs B').
 Proof.
-  intros B B' Hr. induction Hr; sets.
+  intros B B' m Hr. induction Hr; sets.
   rewrite (split_fds_name_in_fundefs _ _ _ H0).
   simpl. sets.
 Qed.
 
 
 Lemma Erase_fundefs_funnames_in_exp : 
-      (forall e e' B (Herase : Erase_fundefs e e' B),
+      (forall e e' B m (Herase : Erase_fundefs e e' B m),
           funnames_in_exp e \subset name_in_fundefs B) /\
-      (forall B B' (Herase : Erase_nested_fundefs B B'),
+      (forall B B' m (Herase : Erase_nested_fundefs B B' m),
           funnames_in_fundefs B \subset name_in_fundefs B').
 Proof.
   exp_defs_induction IHe IHc IHB; intros; simpl; inv Herase;
     try now (intros z Hin; inv Hin; destructAll; inv H; eapply IHe; eauto;
              econstructor; split; eauto).
   - intros x Hin; inv Hin; destructAll. inv H. inv H5.
-  - eapply IHc in H5. intros z Hin; inv Hin; destructAll. inv H. inv H8.
-    + inv H. eapply IHe in H6. erewrite split_fds_name_in_fundefs; [| eassumption ].
-      right; eauto. eapply H6. econstructor. split; eauto.
+  - eapply IHc in H6. intros z Hin; inv Hin; destructAll. inv H. inv H5.
+    + inv H. eapply IHe in H7. erewrite split_fds_name_in_fundefs; [| eassumption ].
+      right; eauto. eapply H7. econstructor. split; eauto.
     + erewrite split_fds_name_in_fundefs; [| eassumption ]. left.
-      eapply H5. econstructor. split; [| eassumption ].
+      eapply H6. econstructor. split; [| eassumption ].
       econstructor. eassumption. eassumption.
   - intros z Hin; inv Hin; destructAll. erewrite split_fds_name_in_fundefs; [| eassumption ]. inv H.
     + right. eapply Erase_nested_fundefs_name_in_fundefs. eassumption. eassumption.
@@ -520,8 +522,8 @@ Proof.
 Qed.
 
 
-Lemma Erase_fundefs_fun_fv_in e e' B
-      (Herase : Erase_fundefs e e' B)
+Lemma Erase_fundefs_fun_fv_in e e' B m
+      (Herase : Erase_fundefs e e' B m)
       (Hsub : fun_fv_in e (funnames_in_exp e)) :  
       fun_fv_in e (name_in_fundefs B).
 Proof.
@@ -531,8 +533,8 @@ Qed.
 
 
 Lemma Erase_fundefs_occurs_free :
-  (forall e e' Ball B Bprev
-          (Herase : Erase_fundefs e e' B)
+  (forall e e' Ball B Bprev m
+          (Herase : Erase_fundefs e e' B m)
           (Hsplit: split_fds Bprev B Ball)
           (Hfv : fun_fv_in e (name_in_fundefs Ball)),
       occurs_free e' \subset (name_in_fundefs Ball) :|: occurs_free e).
@@ -548,16 +550,17 @@ Proof.
     
     eapply Union_Included. now sets.
     eapply Union_Included.    
-    + edestruct split_fds_trans. eapply split_fds_sym. eapply H7. eapply split_fds_sym. eassumption. destructAll.     
-      eapply IHe in H6. 3:{ intros B1 Hin1. eapply Hfv; eauto. econstructor. eassumption. now left. }
+    + edestruct split_fds_trans. eapply split_fds_sym.
+      eapply H8. eapply split_fds_sym. eassumption. destructAll.     
+      eapply IHe in H7. 3:{ intros B1 Hin1. eapply Hfv; eauto. econstructor. eassumption. now left. }
       eapply Included_trans. eassumption. now sets.
       eapply split_fds_sym. eassumption.
-    + edestruct split_fds_trans. eapply H7. eapply split_fds_sym. eassumption. destructAll.     
-      eapply IHe0 in H5.
+    + edestruct split_fds_trans. eapply H8. eapply split_fds_sym. eassumption. destructAll.     
+      eapply IHe0 in H6.
       eapply Included_trans. eassumption. now sets.
       eapply split_fds_sym. eassumption.
       intros B1 Hin1. eapply Hfv; eauto. inv Hin1. econstructor. eassumption. right. eauto. 
-  - edestruct split_fds_trans. eapply H5. eapply split_fds_sym. eassumption. destructAll. 
+  - edestruct split_fds_trans. eapply H6. eapply split_fds_sym. eassumption. destructAll. 
     eapply IHe in H1. 2:{ eapply split_fds_sym. eassumption. }
     2:{ intros B1 Hin1. eapply Hfv; eauto. }
 
@@ -573,13 +576,13 @@ Proof.
 Qed.
 
 Lemma Erase_fundefs_occurs_free_fundefs :
-  (forall e e' Ball B Bprev
-          (Herase : Erase_fundefs e e' B)
+  (forall e e' Ball B Bprev m
+          (Herase : Erase_fundefs e e' B m)
           (Hsplit: split_fds Bprev B Ball)
           (Hfv : fun_fv_in e (name_in_fundefs Ball)),
       occurs_free_fundefs B \subset name_in_fundefs Ball) /\
-  (forall B B' Ball Bprev
-          (Herase : Erase_nested_fundefs B B')
+  (forall B B' Ball Bprev m
+          (Herase : Erase_nested_fundefs B B' m)
           (Hsplit: split_fds Bprev B' Ball)
           (Hfv : fun_fv_in_fundefs B (name_in_fundefs Ball)),
       occurs_free_fundefs B' \subset name_in_fundefs Ball).
@@ -590,21 +593,21 @@ Proof.
   - repeat normalize_occurs_free. sets.
   - rewrite split_fds_occurs_free_fundefs; [| eassumption ].
     eapply Union_Included; eapply Setminus_Included_Included_Union.
-    + edestruct split_fds_trans. eapply H7. eapply split_fds_sym. eassumption. destructAll.
+    + edestruct split_fds_trans. eapply H8. eapply split_fds_sym. eassumption. destructAll.
       eapply Included_trans. eapply IHl. eassumption. eapply split_fds_sym. eassumption.
       intros B1 Hin1. eapply Hfv; eauto. inv Hin1. econstructor. eassumption. right. now eauto.
       now sets.
-    + edestruct split_fds_trans. eapply split_fds_sym. eapply H7. eapply split_fds_sym. eassumption. destructAll.
+    + edestruct split_fds_trans. eapply split_fds_sym. eapply H8. eapply split_fds_sym. eassumption. destructAll.
       eapply Included_trans. eapply IHe. eassumption. eapply split_fds_sym. eassumption.
       intros B1 Hin1. eapply Hfv; eauto. econstructor. eassumption. now left.
       now sets.
   - rewrite split_fds_occurs_free_fundefs; [| eassumption ].
     eapply Union_Included; eapply Setminus_Included_Included_Union.
-    + edestruct split_fds_trans. eapply H5. eapply split_fds_sym. eassumption. destructAll. 
+    + edestruct split_fds_trans. eapply H6. eapply split_fds_sym. eassumption. destructAll. 
       eapply IHe in H1. 2:{ eapply split_fds_sym. eassumption. }
       2:{ intros B1 Hin1. eapply Hfv; eauto. }
       eapply Included_trans. eassumption. sets.
-    + edestruct split_fds_trans. eapply split_fds_sym. eapply H5. eapply split_fds_sym. eassumption. destructAll.
+    + edestruct split_fds_trans. eapply split_fds_sym. eapply H6. eapply split_fds_sym. eassumption. destructAll.
       eapply Included_trans. eapply IHB. eassumption. eapply split_fds_sym. eassumption.
       { intros B1 Hin1. inv Hin1. eapply Hfv; eauto. eapply Hfv; eauto. }
       now sets.
@@ -612,11 +615,11 @@ Proof.
   - normalize_occurs_free. sets.
   - rewrite split_fds_occurs_free_fundefs; [| eassumption ].
     eapply Union_Included; eapply Setminus_Included_Included_Union.
-    + edestruct split_fds_trans. eapply H7. eapply split_fds_sym. eassumption. destructAll. 
+    + edestruct split_fds_trans. eapply H8. eapply split_fds_sym. eassumption. destructAll. 
       eapply Included_trans. eapply IHe. eassumption. eapply split_fds_sym. eassumption.
       intros B1 Hin1. eapply Hfv; eauto. now sets.
     +  normalize_occurs_free. eapply Union_Included; eapply Setminus_Included_Included_Union.
-      * edestruct split_fds_trans. eapply H7. eapply split_fds_sym. eassumption. destructAll.      
+      * edestruct split_fds_trans. eapply H8. eapply split_fds_sym. eassumption. destructAll.      
         eapply Included_trans. eapply Erase_fundefs_occurs_free. eassumption. 
         eapply split_fds_sym. eassumption. intros B1 Hin1. eapply Hfv; eauto.
         eapply Union_Included. now sets.
@@ -632,7 +635,7 @@ Proof.
         
         edestruct split_fds_trans with (B1 := B'0) (B3 := Ball).
         2:{ eapply split_fds_sym. eassumption. } eassumption. destructAll.
-        eapply IHB in H6. 2:{ eapply split_fds_sym. eassumption. }
+        eapply IHB in H7. 2:{ eapply split_fds_sym. eassumption. }
         eapply Included_trans. eassumption. now sets.
         
         intros B1 Hin1. inv Hin1. 2:{ eapply Hfv; eauto. }
@@ -641,7 +644,7 @@ Proof.
         eapply Union_Included.
         -- eapply Included_trans; [| eapply Hfv ]; [| now left ]. normalize_occurs_free. sets.
         -- rewrite split_fds_name_in_fundefs; [| eapply Hsplit ].
-           rewrite split_fds_name_in_fundefs with (B3 := B'); [| eapply H7 ].
+           rewrite split_fds_name_in_fundefs with (B3 := B'); [| eapply H8 ].
            now sets.
   - normalize_occurs_free. sets.
 Qed.
@@ -649,7 +652,7 @@ Qed.
 
 
 Lemma Erase_fundefs_unique_bindings :
-  forall e e' B (Herase : Erase_fundefs e e' B),
+  forall e e' B m (Herase : Erase_fundefs e e' B m),
     unique_bindings e ->
     unique_bindings e' /\
     unique_bindings_fundefs B /\
@@ -657,21 +660,21 @@ Lemma Erase_fundefs_unique_bindings :
 Proof. eapply Erase_fundefs_unique_bindings_mut. Qed.
 
 Lemma Erase_nested_fundefs_unique_bindings :
-  forall B B' (Herase : Erase_nested_fundefs B B'),
+  forall B B' m (Herase : Erase_nested_fundefs B B' m),
     unique_bindings_fundefs B ->
     unique_bindings_fundefs B'.
 Proof. eapply Erase_fundefs_unique_bindings_mut. Qed.   
 
 
-Lemma Erase_nested_fundefs_in_name B B_hoist f tau xs e :
+Lemma Erase_nested_fundefs_in_name B B_hoist f tau xs e m :
   unique_bindings_fundefs B ->
   f \in name_in_fundefs B ->  
-  Erase_nested_fundefs B B_hoist ->
+  Erase_nested_fundefs B B_hoist m ->
   find_def f B = Some (tau, xs, e) ->
-  exists e' Be Bfuns,
+  exists e' Be Bfuns n,
     find_def f B_hoist = Some (tau, xs, e') /\
-    Erase_fundefs e e' Be /\
-    split_fds Be Bfuns B_hoist.
+    Erase_fundefs e e' Be n /\
+    split_fds Be Bfuns B_hoist /\ n <= m.
 Proof.
   intros Hun Hin Hhoist Hfind.
   induction Hhoist. 
@@ -681,15 +684,15 @@ Proof.
     inv Hun.
     destruct (peq f f0).
     * subst. simpl in Hfind. rewrite peq_true in Hfind. inv Hfind.
-      do 3 eexists. split; [| split ].
+      do 4 eexists. split; [| split; [| split ]].
       erewrite split_fds_find_def; [ | | eassumption | ].
       simpl. rewrite peq_true. reflexivity.
       eapply unique_bindings_fundefs_unique_functions.
       eassumption. now left. eassumption.
-      eassumption.
+      eassumption. eapply Nat.le_max_l.
     * subst. simpl in Hfind. rewrite peq_false in Hfind; eauto.
       inv Hin. inv H1; congruence. 
-      edestruct IHHhoist as [e'' [Be' [Bfuns' [Hfind' [Hr Hsplit]]]]];
+      edestruct IHHhoist as [e'' [Be' [Bfuns' [n1 [Hfind' [Hr [Hsplit Hleq]]]]]]];
         eauto.
       assert (Hfind'' : find_def f B'' = Some (tau, xs, e'')).
       { erewrite split_fds_find_def; [ | | eassumption | ].
@@ -697,12 +700,13 @@ Proof.
         eapply unique_bindings_fundefs_unique_functions. eassumption.
         right. eapply Erase_nested_fundefs_name_in_fundefs. eassumption. eassumption. }
       edestruct split_fds_trans as [Bf [Heq1 Heq2]];
-        [| eapply split_fds_sym; eapply H0 | ].        
+        [| eapply split_fds_sym; eapply H0 | ].         
       eapply Right_f; eassumption.
-      do 3 eexists. split; [| split ].
+      do 4 eexists. split; [| split; [| split ]].
       -- eassumption.
       -- eassumption.
       -- eassumption.
+      -- eapply le_trans. eassumption. eapply Nat.le_max_r. 
   - inv Hfind.
 Qed.
   
@@ -718,33 +722,34 @@ Proof.
   - inv Hf2.
 Qed. 
 
-Lemma Erase_fundefs_Ecase x l1 l2 B :
-  Erase_fundefs (Ecase x l1) (Ecase x l2) B ->
+Lemma Erase_fundefs_Ecase x l1 l2 B n :
+  Erase_fundefs (Ecase x l1) (Ecase x l2) B n ->
   Forall2 (fun p1 p2 => fst p1 = fst p2) l1 l2.
 Proof.
-  revert x l2 B; induction l1; intros x l2 B Herase; inv Herase; eauto.
+  revert x l2 B n; induction l1; intros x l2 B n Herase; inv Herase; eauto.
 Qed.
   
   
 Section Hoisting_correct.
   
-  Variable (pr : prims) (cenv : ctor_env). 
+  Variable (pr : prims) (cenv : ctor_env) (G : nat). 
 
   Context {fuel : Type} {Hfuel : @fuel_resource fuel} {trace : Type} {Htrace : @trace_resource trace}.
-
-  Context (P1 : PostT) (* Local *)
+  
+  Context (P1 : nat -> PostT) (* Local *)
           (PG : PostGT) (* Global *)
-          (HP : Post_properties cenv P1 P1 PG)
-          (Hpost_Efun_l : post_Efun_l P1 P1).
+          (HP : forall n, n <= G -> Post_properties cenv (P1 n) (P1 n) PG)
+          (HPmon : forall n m, n <= m -> inclusion _ (P1 n) (P1 m))
+          (Hpost_Efun_l : forall n, post_Efun_l (P1 n) (P1 (S n))).
 
 
   (** * Correctness of Erase_nested_fundefs *)
-  Lemma Erase_nested_fundefs_correct S k B rho rho' B_hoist Bprev Ball
+  Lemma Erase_nested_fundefs_correct S k B rho rho' B_hoist Bprev Ball n (Hleq : n <= G)
         (* IH for expresssions *)
         (IHe :
            forall m : nat,
              m < k ->
-             forall (e e' : exp) (Bprev B Ball : fundefs) (rho rho' : env) (U L : nat),
+             forall (e e' : exp) (Bprev B Ball : fundefs) n (Hleq : n <= G) (rho rho' : env) (U L : nat),
                unique_bindings_fundefs Ball ->
                unique_bindings e ->
                preord_env_P cenv PG (occurs_free e) m rho rho' ->
@@ -752,7 +757,7 @@ Section Hoisting_correct.
                split_fds Bprev B Ball ->
                Disjoint var (name_in_fundefs Ball) (bound_var e') ->
                fun_fv_in e (name_in_fundefs Ball) ->
-               Erase_fundefs e e' B -> preord_exp cenv P1 PG m (e, rho) (e', rho')) :
+               Erase_fundefs e e' B n -> preord_exp cenv (P1 n) PG m (e, rho) (e', rho')) :
     unique_bindings_fundefs Ball ->
     unique_bindings_fundefs B ->
     occurs_free_fundefs B \subset S ->
@@ -764,14 +769,14 @@ Section Hoisting_correct.
     Disjoint var (name_in_fundefs Ball) (bound_var_fundefs B_hoist \\ name_in_fundefs B_hoist) ->
     fun_fv_in_fundefs B (name_in_fundefs Ball) ->
     (* Erase fundefs *)
-    Erase_nested_fundefs B B_hoist ->
+    Erase_nested_fundefs B B_hoist n ->
     (* Environments after defining the function bundles *)
     preord_env_P cenv PG (name_in_fundefs B :|: S) k (def_funs B B rho rho) rho'.
   Proof.
-    revert S B rho rho' B_hoist Bprev Ball IHe.
+    revert S B n Hleq rho rho' B_hoist Bprev Ball IHe.
     induction k as [k IHk] using lt_wf_rec1.
-    intros S B rho rho' B_hoist Bprev Ball IHe Hun1 Hun2 
-           Hsub Henv Hfuns Hsplit Hdis Hfvs Hhoist. assert (Hd' := HP). destruct Hd'.  
+    intros S B n Hleq rho rho' B_hoist Bprev Ball IHe Hun1 Hun2 
+           Hsub Henv Hfuns Hsplit Hdis Hfvs Hhoist. assert (Hd' := HP). edestruct (Hd' n). eassumption.
     rewrite <- (Union_Setminus_Included (name_in_fundefs B) S (name_in_fundefs B)) at 1;
       [| tci | reflexivity ]. 
     eapply preord_env_P_union.
@@ -788,7 +793,7 @@ Section Hoisting_correct.
       
       rewrite preord_val_eq. 
       intros vs1 vs2 j t xs1 e1 rho1' Heq1 Hf1 Hset1.
-      edestruct Erase_nested_fundefs_in_name as [e2' [B2 [B2f [Hf2 [Hr2 Hs2]]]]];
+      edestruct Erase_nested_fundefs_in_name as [e2' [B2 [B2f [n1 [Hf2 [Hr2 [Hs2 Hleq']]]]]]];
         [| | | eapply Hf1 | ]; eauto.
       edestruct (@set_lists_length3 val (def_funs Ball Ball rhoi rhoi) xs1 vs2)
         as [rho2' Hset2].
@@ -799,13 +804,14 @@ Section Hoisting_correct.
         eapply Erase_nested_fundefs_name_in_fundefs; eassumption.
       + eauto.
       + intros Hlt Hall.
-        eapply preord_exp_post_monotonic with (P1 := P1). eassumption.
+        eapply preord_exp_post_monotonic with (P1 := P1 n1). eapply Hd'. omega.
 
         assert (Hsplit' := Hsplit).
         eapply split_fds_sym in Hsplit.
         edestruct (split_fds_trans _ _ _ _ _ Hs2 Hsplit) as [Bprev' [Hs3 Hs4]].
         eapply IHe with (Ball := Ball) (Bprev := Bprev');
           last eassumption; try eassumption.
+        * omega.
         * eapply unique_bindings_fun_in_fundefs.
           eapply find_def_correct. eassumption.
           eassumption.
@@ -857,9 +863,11 @@ Section Hoisting_correct.
       eapply preord_env_P_antimon. eassumption. sets.
   Qed.
 
+  Require Import Coq.micromega.Lia. 
+
   (** * Correctness of Erase_fundefs *)
   
-  Lemma hoisting_correct k e e' Bprev B Ball rho rho' :
+  Lemma hoisting_correct k e e' Bprev B Ball rho rho' n (Hleq : n <= G) :
     unique_bindings_fundefs Ball ->
     unique_bindings e ->
     (* environments are related *)
@@ -872,22 +880,22 @@ Section Hoisting_correct.
     (* the FVs of the original functions are in the global fundefs *)
     fun_fv_in e (name_in_fundefs Ball) ->
     (* Hoisting *)            
-    Erase_fundefs e e' B ->    
-    preord_exp cenv P1 PG k (e, rho) (e', rho').
+    Erase_fundefs e e' B n ->    
+    preord_exp cenv (P1 n) PG k (e, rho) (e', rho').
   Proof.
-    revert e e' Bprev B Ball rho rho'.
+    revert e e' Bprev B Ball n Hleq rho rho'.
     induction k as [k IHk] using lt_wf_rec1.
     intros e; revert k IHk; induction e using exp_ind';
-    intros k IHk e' Bprev B Ball rho rho' Hun1 Hun2 Henv Hfuns Hsplit Hdis Hfvs Hhoist;
-      inv Hhoist; inv Hun2; assert (Hd' := HP); destruct Hd'.
+      intros k IHk e' Bprev B Ball m Hleq' rho rho' Hun1 Hun2 Henv Hfuns Hsplit Hdis Hfvs Hhoist;
+      inv Hhoist; inv Hun2; try (assert (Hd' := HP m); destruct Hd'; try omega).
     - (* Econstr *)
       eapply preord_exp_constr_compat.
       + now eauto.
       + now eauto.
       + eapply Forall2_same. intros x Hin. eapply Henv.
         now constructor.
-      + intros m vs1 vs2 Hlt Hall. 
-        eapply IHk; [ eassumption | eassumption | | | | eassumption | | | ].
+      + intros m1 vs1 vs2 Hlt Hall. 
+        eapply IHk; [ eassumption | eassumption | eassumption | | | | eassumption | | | ].
         * eassumption.
         * eapply preord_env_P_extend.
           -- eapply preord_env_P_antimon.
@@ -903,17 +911,23 @@ Section Hoisting_correct.
         * intros B' Hbin. eapply Hfvs. constructor; eauto.
         * eassumption.
     - (* Ecase nil *)
-      eapply preord_exp_case_nil_compat. now eauto.
+      eapply preord_exp_case_nil_compat. eapply HP. omega.
     - (* Ecase cons *)
-      eapply split_fds_sym in H7.
+      eapply split_fds_sym in H8.
       edestruct split_fds_trans as [Bnew [Hs1 Hs2]].
-      now eapply H7. eapply split_fds_sym. eassumption.
-      eapply split_fds_sym in H7.
+      now eapply H8. eapply split_fds_sym. eassumption.
+      eapply split_fds_sym in H8.
       edestruct split_fds_trans as [Bnew' [Hs1' Hs2']].
-      now eapply H7. eapply split_fds_sym. eassumption.      
+      now eapply H8. eapply split_fds_sym. eassumption.      
       eapply preord_exp_case_cons_compat; eauto.
+      + eapply HP. omega.
+      + eapply HP. omega.
+      + eapply HP. omega.
       + eapply Erase_fundefs_Ecase. eassumption.
-      + intros m Hlt. eapply IHk; last eassumption; eauto.
+      + intros m Hlt.
+        eapply preord_exp_post_monotonic. eapply HPmon with (n := m0). lia.
+        eapply IHk; last eassumption; eauto.
+        * lia.
         * eapply preord_env_P_antimon.
           eapply preord_env_P_monotonic; [| eassumption ]. omega.
           normalize_occurs_free; sets.
@@ -922,7 +936,9 @@ Section Hoisting_correct.
           normalize_bound_var; sets.
         * intros x Hin; eapply Hfvs. econstructor; eauto.
           now left.
-      + eapply IHe0; last eassumption; eauto.
+      + eapply preord_exp_post_monotonic. eapply HPmon with (n := n). lia.
+        eapply IHe0; last eassumption; eauto.
+        * lia.
         * eapply preord_env_P_antimon. eassumption.
           normalize_occurs_free; sets.
         * apply split_fds_sym. eassumption.
@@ -936,8 +952,8 @@ Section Hoisting_correct.
       + now eauto.
       + now eauto. 
       + eapply Henv. eauto.
-      + intros m vs1 vs2 Hlt Hall. 
-        eapply IHk; [ eassumption | eassumption | | | | eassumption | | | ].
+      + intros m1 vs1 vs2 Hlt Hall. 
+        eapply IHk; [ eassumption | eassumption | eassumption | | | | eassumption | | | ].
         * eassumption.
         * eapply preord_env_P_extend.
           -- eapply preord_env_P_antimon.
@@ -959,8 +975,8 @@ Section Hoisting_correct.
       + eapply Henv. constructor. now left.
       + eapply Forall2_same. intros z Hin. eapply Henv.
         constructor. now right.
-      + intros m v1 v2 hlew Hrel.
-        eapply IHk; [ eassumption | eassumption | | | | eassumption | | | ].
+      + intros m1 v1 v2 hlew Hrel.
+        eapply IHk; [ eassumption | eassumption | eassumption | | | | eassumption | | | ].
         * eassumption.
         * eapply preord_env_P_extend.
           -- eapply preord_env_P_antimon.
@@ -976,19 +992,22 @@ Section Hoisting_correct.
         * eassumption.
     - (* Efun -- the only non trivial case *)
       eapply preord_exp_Efun_l.
+      + eapply HP. lia. 
       + now eauto.
-      + eapply Hpost_Efun_l.
       + eapply split_fds_sym in Hsplit.
-        eapply split_fds_sym in H5.
-        edestruct split_fds_trans as [Bnew [Hs1 Hs2]]. now eapply H5. eassumption.        
-        eapply split_fds_sym in H5.
-        edestruct split_fds_trans as [Bnew' [Hs1' Hs2']]. now eapply H5. eassumption.
-                         
-        eapply IHe with (Ball := Ball); [ | eassumption | eassumption | | | | | | eassumption ].
+        eapply split_fds_sym in H6.
+        edestruct split_fds_trans as [Bnew [Hs1 Hs2]]. now eapply H6. eassumption.        
+        eapply split_fds_sym in H6.
+        edestruct split_fds_trans as [Bnew' [Hs1' Hs2']]. now eapply H6. eassumption.
+        eapply preord_exp_post_monotonic. eapply HPmon with (n := n). lia.
+                                  
+        eapply IHe with (Ball := Ball); [ | | eassumption | eassumption | | | | | | eassumption ].
         * intros. eapply IHk; eauto. omega.
+        * lia. 
         * eapply preord_env_P_antimon.
           -- { eapply Erase_nested_fundefs_correct with (S := occurs_free_fundefs f2 :|: occurs_free e);
-               [ | | | | | | | | | eassumption ].
+               [ | | | | | | | | | | eassumption ].
+               - lia. 
                - intros. eapply IHk; eauto. omega.
                - eapply Hun1.
                - eassumption.
@@ -1016,8 +1035,8 @@ Section Hoisting_correct.
         * intros x Hin. eapply Hfvs. constructor; eauto.
     - (* Eapp *)
       eapply preord_exp_app_compat.
-      + now eauto.
-      + now eauto.
+      + eapply HP. lia.
+      + eapply HP. lia.
       + eapply Henv. constructor.
       + eapply Forall2_same. intros z Hin. eapply Henv.
         now constructor.
@@ -1027,7 +1046,9 @@ Section Hoisting_correct.
       + eapply Forall2_same. intros x Hin. eapply Henv.
         now constructor.
     - (* Ehalt *)
-      eapply preord_exp_halt_compat; eauto. 
+      eapply preord_exp_halt_compat; eauto.
+      + eapply HP. lia.
+      + eapply HP. lia.
   Qed.
 
 
@@ -1037,14 +1058,14 @@ Section Hoisting_correct.
 
   Context (P2: @PostT fuel trace). 
 
-  Context (Hp2 : post_Efun_r P1 P2) (Hoot2 : post_OOT P2). 
+  Context (Hp2 : forall n, n <= G -> post_Efun_r (P1 n) P2) (Hoot2 : post_OOT P2). 
   
-  Lemma Erase_fundefs_correct_top k e e' B :
+  Lemma Erase_fundefs_correct_top k e e' B n (Hleq : n <= G) :
     unique_bindings e ->
     Disjoint _ (occurs_free e) (bound_var e) ->
     fun_fv_in e (funnames_in_exp e) ->
     (* Hoisting *)            
-    Erase_fundefs e e' B ->
+    Erase_fundefs e e' B n ->
 
     (forall rho rho',
         preord_env_P cenv PG (occurs_free e) k rho rho' ->
@@ -1056,9 +1077,10 @@ Section Hoisting_correct.
     { intros rho rho' Henv. 
       eapply preord_exp_Efun_r.
       - eassumption.
-      - eassumption.
+      - eauto.
       - edestruct Erase_fundefs_unique_bindings. eassumption. eassumption. destructAll.
         eapply hoisting_correct with (Bprev := Fnil) (B := B) (Ball := B).
+        + omega. 
         + eassumption.
         + eassumption.
         + eapply preord_env_P_def_funs_not_in_P_r. eassumption. 
@@ -1091,14 +1113,14 @@ Section Hoisting_correct.
         sets. }
   Qed.
 
-  Context (Hinc : inclusion (exp * env * fuel * trace) P1 P2).
+  Context (Hinc : forall n, n <= G -> inclusion (exp * env * fuel * trace) (P1 n) P2).
   
-  Lemma Erase_fundefs_correct_top_Fnil k e e' :
+  Lemma Erase_fundefs_correct_top_Fnil k e e' n (Hleq : n <= G) :
     unique_bindings e ->
     Disjoint _ (occurs_free e) (bound_var e) ->
     fun_fv_in e (funnames_in_exp e) ->
     (* Hoisting *)            
-    Erase_fundefs e e' Fnil ->
+    Erase_fundefs e e' Fnil n ->
 
     (forall rho rho',
         preord_env_P cenv PG (occurs_free e) k rho rho' ->
@@ -1117,8 +1139,9 @@ Section Hoisting_correct.
     intros rho rho' Henv. 
 
     edestruct Erase_fundefs_unique_bindings. eassumption. eassumption. destructAll.
-    eapply preord_exp_post_monotonic. eapply Hinc.
+    eapply preord_exp_post_monotonic. eapply Hinc. eassumption. 
     eapply hoisting_correct with (Bprev := Fnil) (B := Fnil) (Ball := Fnil).
+    + eassumption.
     + eassumption.
     + eassumption.
     + eassumption.
@@ -1131,12 +1154,12 @@ Section Hoisting_correct.
       Grab Existential Variables. exact 1.
   Qed.
 
-  Lemma exp_hoist_correct_top k e e' :
+  Lemma exp_hoist_correct_top k e e' n (Hleq : n <= G) :
     unique_bindings e ->
     Disjoint _ (occurs_free e) (bound_var e) ->
     fun_fv_in e (funnames_in_exp e) ->
     
-    exp_hoist e = e' -> 
+    exp_hoist e = (e', n) -> 
 
     (forall rho rho',
         preord_env_P cenv PG (occurs_free e) k rho rho' ->
@@ -1147,12 +1170,12 @@ Section Hoisting_correct.
     intros Hun Hdis Hfv Hh.
     unfold exp_hoist in Hh.
 
-    edestruct (proj1 erase_fundefs_in_Erase_fundefs) as [e1 [B1 [B2 [H1 [Hs H2]]]]].
+    edestruct (proj1 erase_fundefs_in_Erase_fundefs) as [e1 [B1 [B2 [m [H1 [Hs H2]]]]]].
     rewrite H1 in Hh. unfold id in *. clear H1.
     eapply split_fds_Fnil_eq_l in Hs. rewrite Hs in *. clear Hs. 
     destruct B1.
-    - subst. eapply Erase_fundefs_correct_top; eauto.
-    - subst. eapply Erase_fundefs_correct_top_Fnil; eauto.
+    - inv Hh. eapply Erase_fundefs_correct_top; eauto.
+    - inv Hh. eapply Erase_fundefs_correct_top_Fnil; eauto.
   Qed.
     
 End Hoisting_correct.
